Renaming subtyping

CC/Basic.lean
@@ -4,10 +4,48 @@ namespace CC
 
 def VarMap (n m : Nat) : Type := Fin n -> Fin m
 
-def extv (f : VarMap n m) : VarMap n.succ m.succ := by
+def VarMap.ext (f : VarMap n m) : VarMap n.succ m.succ := by
   intro i
   cases i using Fin.cases with
   | H0 => exact 0
   | Hs i0 => exact (f i0).succ
 
+def VarMap.comp (f : VarMap n2 n3) (f' : VarMap n1 n2) : VarMap n1 n3 := Function.comp f f'
+
 def weaken_map : VarMap n n.succ := fun x => x.succ
+
+def open_map (k : Fin n) : VarMap n.succ n := by
+  intro i
+  cases i using Fin.cases with
+  | H0 => exact k
+  | Hs i0 => exact i0
+
+@[simp]
+theorem id_ext : VarMap.ext (n := n) id = id := by
+  unfold VarMap
+  ext x
+  cases x using Fin.cases <;> aesop
+
+theorem ext_comp {f1 : VarMap n1 n2} {f2 : VarMap n2 n3} :
+  VarMap.ext (f2.comp f1) = f2.ext.comp f1.ext := by
+  unfold VarMap
+  ext x0
+  cases x0 using Fin.cases <;> aesop
+
+@[simp]
+theorem comp_id (f : VarMap n1 n2) :
+  f.comp id = f := by
+  unfold VarMap
+  ext x0
+  simp [VarMap.comp]
+
+@[simp]
+theorem id_comp (f : VarMap n1 n2) :
+  VarMap.comp id f = f := by
+  unfold VarMap
+  ext x0
+  simp [VarMap.comp]
+
+@[simp]
+theorem ext_comp_weaken (f : VarMap n1 n2) :
+  f.ext.comp weaken_map = weaken_map.comp f := by aesop
