CC/Type.lean
@@ -25,9 +25,9 @@ def PType.rename (S : PType n1 m1) (f : VarMap n1 n2) (g : VarMap m1 m2) : PType
   | PType.tvar x => PType.tvar (g x)
   | PType.top => PType.top
   | PType.arr (CType.capt C1 S1) (CType.capt C2 S2) => 
-    PType.arr (CType.capt (C1.rename f) (S1.rename f g)) (CType.capt (C2.rename (extv f)) (S2.rename (extv f) g))
+    PType.arr (CType.capt (C1.rename f) (S1.rename f g)) (CType.capt (C2.rename f.ext) (S2.rename f.ext g))
   | PType.tarr S (CType.capt C R) => 
-    PType.tarr (S.rename f g) (CType.capt (C.rename f) (R.rename f (extv g)))
+    PType.tarr (S.rename f g) (CType.capt (C.rename f) (R.rename f g.ext))
   | PType.boxed (CType.capt C R) => PType.boxed (CType.capt (C.rename f) (R.rename f g))
 
 def CType.rename (T : CType n1 m1) (f : VarMap n1 n2) (g : VarMap m1 m2) : CType n2 m2 :=
@@ -45,3 +45,82 @@ def CType.weaken_var (T : CType n m) : CType n.succ m :=
 
 def CType.weaken_tvar (T : CType n m) : CType n m.succ :=
   T.rename id weaken_map
+
+@[simp]
+theorem rename_capt :
+  (CType.capt C S).rename f g = CType.capt (C.rename f) (S.rename f g) :=
+  rfl
+
+@[simp]
+theorem rename_arr :
+  (PType.arr T1 T2).rename f g = PType.arr (T1.rename f g) (T2.rename f.ext g) := by
+  cases T1
+  cases T2
+  simp [PType.rename]
+
+@[simp]
+theorem rename_tarr :
+  (PType.tarr T1 T2).rename f g = PType.tarr (T1.rename f g) (T2.rename f g.ext) := by
+  cases T2
+  simp [PType.rename]
+
+@[simp]
+theorem rename_boxed :
+  (PType.boxed T).rename f g = PType.boxed (T.rename f g) := by
+  cases T
+  simp [PType.rename]
+
+@[simp]
+theorem PType.rename_id : (S : PType n m) -> S.rename id id = S
+| PType.tvar x => by simp [PType.rename]
+| PType.top => by simp [PType.rename]
+| PType.arr (CType.capt C1 S1) (CType.capt C2 S2) => by
+  simp [PType.rename]
+  have ih1 := PType.rename_id S1
+  have ih2 := PType.rename_id S2
+  aesop
+| PType.tarr S (CType.capt C R) => by
+  simp [PType.rename]
+  have ih1 := PType.rename_id S
+  have ih2 := PType.rename_id R
+  aesop
+| PType.boxed (CType.capt C R) => by
+  simp [PType.rename]
+  have ih := PType.rename_id R; aesop
+
+@[simp]
+theorem CType.rename_id : (T : CType n m) -> T.rename id id = T
+| CType.capt C S => by
+  simp [CType.rename]
+
+theorem PType.rename_comp
+  {f1 : VarMap n1 n2} {f2 : VarMap n2 n3}
+  {g1 : VarMap m1 m2} {g2 : VarMap m2 m3} :
+  (S : PType n1 m1) ->
+  (S.rename f1 g1).rename f2 g2 = S.rename (f2.comp f1) (g2.comp g1)
+| PType.tvar X => by
+  unfold VarMap.comp
+  simp [PType.rename]
+| PType.top => by simp [PType.rename]
+| PType.arr (CType.capt C1 S1) (CType.capt C2 S2) => by
+  simp [PType.rename]
+  simp [CaptureSet.rename_comp]
+  simp [ext_comp]
+  apply And.intro <;> apply PType.rename_comp
+| PType.tarr S (CType.capt C R) => by
+  simp [PType.rename]
+  simp [CaptureSet.rename_comp]
+  simp [ext_comp]
+  apply And.intro <;> apply PType.rename_comp
+| PType.boxed (CType.capt C R) => by
+  simp [PType.rename]
+  simp [CaptureSet.rename_comp]
+  apply PType.rename_comp
+
+theorem CType.rename_comp
+  {f1 : VarMap n1 n2} {f2 : VarMap n2 n3}
+  {g1 : VarMap m1 m2} {g2 : VarMap m2 m3} :
+  (T : CType n1 m1) ->
+  (T.rename f1 g1).rename f2 g2 = T.rename (f2.comp f1) (g2.comp g1)
+| CType.capt C R => by
+  simp [CaptureSet.rename_comp, PType.rename_comp]
