CC/CaptureSet.lean
@@ -13,8 +13,50 @@ instance : Membership (Fin n) (CaptureSet n) :=
 instance : Singleton (Fin n) (CaptureSet n) :=
   ⟨fun x => ⟨{x}⟩⟩ 
 
+instance : Union (CaptureSet n) :=
+  ⟨fun s t => ⟨s.1 ∪ t.1⟩⟩ 
+
 def CaptureSet.rename (C : CaptureSet n1) (f : VarMap n1 n2) : CaptureSet n2 :=
-  ⟨C.elems.image f⟩  
+  ⟨C.elems.image f⟩
   
 def CaptureSet.weaken_var (C : CaptureSet n) : CaptureSet n.succ :=
   C.rename weaken_map
+
+theorem singleton_val (x : Fin n) :
+  ({x} : CaptureSet n).1 = {x} := rfl
+
+@[simp]
+theorem rename_singleton (x : Fin n) (f : VarMap n n') :
+  CaptureSet.rename {x} f = {f x} := by
+  simp [CaptureSet.rename]
+  aesop
+
+theorem mem_def {x : Fin n} {C : CaptureSet n} : x ∈ C ↔ x ∈ C.1 := Iff.rfl
+
+theorem mem_rename_of_mem (f : VarMap n1 n2) {C : CaptureSet n1} (h : x ∈ C) : f x ∈ C.rename f := by
+  unfold CaptureSet.rename
+  simp [mem_def]
+  aesop
+
+@[simp]
+theorem mem_rename {C : CaptureSet n} :
+  y ∈ C.rename f ↔ ∃ x ∈ C, f x = y := by
+  simp only [CaptureSet.rename, mem_def]
+  aesop
+
+@[simp]
+theorem CaptureSet.rename_id : ∀ {C : CaptureSet n},
+  C.rename id = C := by
+  introv
+  simp [CaptureSet.rename]
+
+@[simp]
+theorem CaptureSet.rename_id' : ∀ {C : CaptureSet n},
+  C.rename (fun x => x) = C := by
+  introv
+  simp [CaptureSet.rename]
+
+theorem CaptureSet.rename_comp {C : CaptureSet n1} {f1 : VarMap n1 n2} {f2 : VarMap n2 n3} :
+  (C.rename f1).rename f2 = C.rename (f2.comp f1) := by
+  unfold VarMap.comp
+  simp [CaptureSet.rename, Finset.image_image]
