CC/Rename.lean
@@ -1,0 +1,105 @@
+import CC.Basic
+import CC.Type
+import CC.Context
+
+namespace CC
+
+def VarRename (Γ : Ctx n1 m1) (Δ : Ctx n2 m2) (f : VarMap n1 n2) (g : VarMap m1 m2) : Prop :=
+  ∀ {x T}, BoundVar Γ x T -> BoundVar Δ (f x) (T.rename f g)
+
+def TVarRename (Γ : Ctx n1 m1) (Δ : Ctx n2 m2) (f : VarMap n1 n2) (g : VarMap m1 m2) : Prop :=
+  ∀ {X S}, BoundTVar Γ X S -> BoundTVar Δ (g X) (S.rename f g)
+
+theorem CType.rename_weaken_var_comp (T : CType n m) :
+  T.weaken_var.rename f g = T.rename (f.comp weaken_map) g := by
+  simp [weaken_var]
+  simp [CType.rename_comp]
+
+theorem CType.rename_weaken_tvar_comp (T : CType n m) :
+  T.weaken_tvar.rename f g = T.rename f (g.comp weaken_map) := by
+  simp [weaken_tvar]
+  simp [CType.rename_comp]
+
+theorem PType.rename_weaken_var_comp (S : PType n m) :
+  S.weaken_var.rename f g = S.rename (f.comp weaken_map) g := by
+  simp [weaken_var]
+  simp [PType.rename_comp]
+
+theorem PType.rename_weaken_tvar_comp (S : PType n m) :
+  S.weaken_tvar.rename f g = S.rename f (g.comp weaken_map) := by
+  simp [weaken_tvar]
+  simp [PType.rename_comp]
+
+theorem CType.weaken_var_rename_comp (T : CType n m) :
+  (T.rename f g).weaken_var = T.rename (weaken_map.comp f) g := by
+  simp [weaken_var]
+  simp [CType.rename_comp]
+
+theorem CType.weaken_tvar_rename_comp (T : CType n m) :
+  (T.rename f g).weaken_tvar = T.rename f (weaken_map.comp g) := by
+  simp [weaken_tvar]
+  simp [CType.rename_comp]
+
+theorem PType.weaken_tvar_rename_comp (S : PType n m) :
+  (S.rename f g).weaken_tvar = S.rename f (weaken_map.comp g) := by
+  simp [weaken_tvar]
+  simp [PType.rename_comp]
+
+theorem PType.weaken_var_rename_comp (S : PType n m) :
+  (S.rename f g).weaken_var = S.rename (weaken_map.comp f) g := by
+  simp [weaken_var]
+  simp [PType.rename_comp]
+
+def VarRename.ext_var {Γ : Ctx n1 m1} {Δ : Ctx n2 m2} 
+  (σ : VarRename Γ Δ f g) (T : CType n1 m1) :
+  VarRename (Ctx.extend_var Γ T) (Ctx.extend_var Δ (T.rename f g)) f.ext g := by
+  intro x P h
+  cases h with
+  | here =>
+    simp [CType.rename_weaken_var_comp]
+    rw [<- CType.weaken_var_rename_comp]
+    simp [VarMap.ext]
+    constructor
+  | there_var h =>
+    simp [CType.rename_weaken_var_comp]
+    rw [<- CType.weaken_var_rename_comp]
+    simp [VarMap.ext]
+    constructor
+    aesop
+
+def VarRename.ext_tvar {Γ : Ctx n1 m1} {Δ : Ctx n2 m2}
+  (σ : VarRename Γ Δ f g) (R : PType n1 m1) :
+  VarRename (Ctx.extend_tvar Γ R) (Ctx.extend_tvar Δ (R.rename f g)) f g.ext := by
+  intro x P h
+  cases h with
+  | there_tvar h =>
+    simp [CType.rename_weaken_tvar_comp]
+    rw [<- CType.weaken_tvar_rename_comp]
+    constructor; aesop
+
+def TVarRename.ext_var {Γ : Ctx n1 m1} {Δ : Ctx n2 m2}
+  (δ : TVarRename Γ Δ f g) (T : CType n1 m1) :
+  TVarRename (Ctx.extend_var Γ T) (Ctx.extend_var Δ (T.rename f g)) f.ext g := by
+  intro X R h
+  cases h with
+  | there_var h =>
+    simp [PType.rename_weaken_var_comp]
+    rw [<- PType.weaken_var_rename_comp]
+    constructor
+    aesop
+
+def TVarRename.ext_tvar {Γ : Ctx n1 m1} {Δ : Ctx n2 m2}
+  (δ : TVarRename Γ Δ f g) (R : PType n1 m1) :
+  TVarRename (Ctx.extend_tvar Γ R) (Ctx.extend_tvar Δ (R.rename f g)) f g.ext := by
+  intro X R h
+  cases h with
+  | here =>
+    simp [PType.rename_weaken_tvar_comp]
+    rw [<- PType.weaken_tvar_rename_comp]
+    simp [VarMap.ext]
+    constructor
+  | there_tvar h =>
+    simp [PType.rename_weaken_tvar_comp]
+    rw [<- PType.weaken_tvar_rename_comp]
+    constructor
+    aesop
