CC/Subcapt/Rename.lean
@@ -1,0 +1,39 @@
+import Mathlib.Data.Finset.Basic
+import Mathlib.Data.Finset.Image
+
+import CC.Basic
+import CC.Rename
+
+import CC.CaptureSet
+import CC.Context
+import CC.Type
+import CC.Subcapt
+
+namespace CC
+
+def Subcapt.rename (σ : VarRename Γ Δ f g) : Subcapt Γ C1 C2 -> Subcapt Δ (C1.rename f) (C2.rename f) := by
+  intro h
+  induction h
+  case sc_trans ih1 ih2 =>
+    apply Subcapt.sc_trans
+    apply ih1; aesop
+    apply ih2; aesop
+  case sc_elem h =>
+    simp
+    apply Subcapt.sc_elem
+    apply mem_rename_of_mem; assumption
+  case sc_var h =>
+    simp
+    apply Subcapt.sc_var
+    have H := σ h
+    simp at H
+    assumption
+  case sc_set hs =>
+    apply Subcapt.sc_set
+    intro x1 h1
+    rw [mem_rename] at h1
+    let ⟨x2, ⟨h2, eq2⟩⟩ := h1
+    have h := hs x2 h2 σ
+    rw [rename_singleton] at h
+    rw [<- eq2]
+    assumption
