CC/Subtype/Rename.lean
@@ -1,0 +1,81 @@
+import Mathlib.Data.Finset.Basic
+import Mathlib.Data.Finset.Image
+
+import CC.Basic
+import CC.Rename
+
+import CC.CaptureSet
+import CC.Context
+import CC.Type
+import CC.Subcapt
+import CC.Subcapt.Rename
+import CC.Subtype
+
+namespace CC
+
+def SubtypeP.rename {Γ : Ctx n1 m1} {Δ : Ctx n2 m2} {T1 T2 : PType n1 m1} 
+  (h : SubtypeP Γ T1 T2)
+  {f : VarMap n1 n2} {g : VarMap m1 m2}
+  (σ : VarRename Γ Δ f g) (δ : TVarRename Γ Δ f g) :
+  SubtypeP Δ (T1.rename f g) (T2.rename f g) := by
+  apply SubtypeP.rec
+        (motive_1 := 
+          fun Γ T1 T2 _ => 
+            ∀ {n2 m2} {Δ : Ctx n2 m2} {f g} (_ : VarRename Γ Δ f g) (_ : TVarRename Γ Δ f g), Subtype Δ (T1.rename f g) (T2.rename f g))
+        (motive_2 :=
+          fun Γ T1 T2 _ => 
+            ∀ {n2 m2} {Δ : Ctx n2 m2} {f g} (_ : VarRename Γ Δ f g) (_ : TVarRename Γ Δ f g), SubtypeP Δ (T1.rename f g) (T2.rename f g))
+    <;> try assumption
+  case capt =>
+    intros; rename_i hc _ ih _ _ _ σ δ
+    simp
+    constructor
+    apply Subcapt.rename <;> aesop
+    aesop
+  case refl =>
+    intros
+    constructor
+  case trans =>
+    intros; rename_i ih1 ih2 _ _ _ σ δ
+    apply SubtypeP.trans <;> aesop
+  case top =>
+    intros
+    simp [PType.rename]
+    apply SubtypeP.top
+  case tvar =>
+    intros; rename_i hb _ _ _ _ δ
+    simp [PType.rename]
+    apply SubtypeP.tvar
+    aesop
+  case arr =>
+    intros; rename_i ih1 ih2 _ _ Δ f g σ δ
+    simp
+    apply SubtypeP.arr
+    aesop
+    apply ih2
+    apply σ.ext_var
+    apply δ.ext_var
+  case tarr =>
+    intros; rename_i ih1 ih2 _ _ Δ f g σ δ
+    simp
+    apply SubtypeP.tarr
+    aesop
+    apply ih2
+    apply σ.ext_tvar
+    apply δ.ext_tvar
+  case boxed =>
+    intros; rename_i ih _ _ Δ f g σ δ
+    simp
+    apply SubtypeP.boxed
+    aesop
+  
+def Subtype.rename {Γ : Ctx n1 m1} {Δ : Ctx n2 m2} {T1 T2 : CType n1 m1} 
+  (h : Subtype Γ T1 T2)
+  {f : VarMap n1 n2} {g : VarMap m1 m2}
+  (σ : VarRename Γ Δ f g) (δ : TVarRename Γ Δ f g) :
+  Subtype Δ (T1.rename f g) (T2.rename f g) := by
+  cases h
+  simp
+  apply Subtype.capt
+  apply Subcapt.rename <;> aesop
+  apply SubtypeP.rename <;> aesop
